One more round of cleanup

src/Std/Data/ExtDTreeMap/Basic.lean
@@ -924,46 +924,28 @@ def inter [TransCmp cmp] (m₁ m₂ : ExtDTreeMap α β cmp) : ExtDTreeMap α β
 
 instance [TransCmp cmp] : Inter (ExtDTreeMap α β cmp) := ⟨inter⟩
 
-@[inline, inherit_doc DTreeMap.beq]
-def beq [LawfulEqCmp cmp] [TransCmp cmp] [∀ k, BEq (β k)] (m₁ m₂ : ExtDTreeMap α β cmp) : Bool := lift₂ (fun x y : DTreeMap α β cmp => x.beq y)
-  (fun _ _ _ _ => DTreeMap.Equiv.beq_congr) m₁ m₂
-
-instance [LawfulEqCmp cmp] [TransCmp cmp] [∀ k, BEq (β k)] : BEq (ExtDTreeMap α β cmp) := ⟨beq⟩
+instance [LawfulEqCmp cmp] [TransCmp cmp] [∀ k, BEq (β k)] : BEq (ExtDTreeMap α β cmp) where
+  beq := lift₂ (fun x y : DTreeMap α β cmp => x.beq y) fun _ _ _ _ => DTreeMap.Equiv.beq_congr
 
 instance [LawfulEqCmp cmp] [TransCmp cmp] [∀ k, BEq (β k)] [∀ k, ReflBEq (β k)] : ReflBEq (ExtDTreeMap α β cmp) where
-  rfl {a} := by
-    induction a
-    case mk a =>
-      apply DTreeMap.Equiv.beq <| DTreeMap.Equiv.rfl
+  rfl {a} := a.inductionOn fun _ => DTreeMap.Equiv.beq <| DTreeMap.Equiv.rfl
 
 instance [LawfulEqCmp cmp] [TransCmp cmp] [∀ k, BEq (β k)] [∀ k, LawfulBEq (β k)] : LawfulBEq (ExtDTreeMap α β cmp) where
-  eq_of_beq {a} {b} hyp := by
-    induction a
-    case mk a =>
-      induction b
-      case mk b =>
-        apply sound <| DTreeMap.equiv_of_beq hyp
+  eq_of_beq {a} {b} := a.inductionOn₂ b fun _ _ h => sound <| DTreeMap.equiv_of_beq h
 
 namespace Const
+
 variable {β : Type v}
 
 @[inline, inherit_doc DTreeMap.beq]
-def beq [TransCmp cmp] [LawfulEqCmp cmp] [BEq β] (m₁ m₂ : ExtDTreeMap α (fun _ => β) cmp) : Bool := lift₂ (fun x y : DTreeMap α (fun _ => β) cmp => DTreeMap.Const.beq x y)
+def beq [TransCmp cmp] [BEq β] (m₁ m₂ : ExtDTreeMap α (fun _ => β) cmp) : Bool := lift₂ (fun x y : DTreeMap α (fun _ => β) cmp => DTreeMap.Const.beq x y)
   (fun _ _ _ _ => DTreeMap.Const.Equiv.beq_congr) m₁ m₂
 
-theorem beq_of_eq [TransCmp cmp] [LawfulEqCmp cmp] [BEq β] [ReflBEq β] (m₁ m₂ : ExtDTreeMap α (fun _ => β) cmp) (h : m₁ = m₂) : Const.beq m₁ m₂ := by
-  induction m₁
-  case mk a =>
-    induction m₂
-    case mk b =>
-      exact DTreeMap.Const.Equiv.beq <| exact h
+theorem beq_of_eq [TransCmp cmp] [BEq β] [ReflBEq β] (m₁ m₂ : ExtDTreeMap α (fun _ => β) cmp) : m₁ = m₂ → Const.beq m₁ m₂ :=
+  m₁.inductionOn₂ m₂ fun _ _ h => DTreeMap.Const.Equiv.beq <| exact h
 
-theorem eq_of_beq [TransCmp cmp] [LawfulEqCmp cmp] [BEq β] [LawfulBEq β] (m₁ m₂ : ExtDTreeMap α (fun _ => β) cmp) (h : Const.beq m₁ m₂) : m₁ = m₂ := by
-  induction m₁
-  case mk a =>
-    induction m₂
-    case mk b =>
-      exact sound <| DTreeMap.Const.equiv_of_beq h
+theorem eq_of_beq [TransCmp cmp] [LawfulEqCmp cmp] [BEq β] [LawfulBEq β] (m₁ m₂ : ExtDTreeMap α (fun _ => β) cmp) : Const.beq m₁ m₂ → m₁ = m₂ :=
+  m₁.inductionOn₂ m₂ fun _ _ h => sound <| DTreeMap.Const.equiv_of_beq h
 
 end Const
 
