src/Std/Data/DTreeMap/Lemmas.lean
@@ -2880,30 +2880,32 @@ theorem get!_inter_of_not_mem_left [TransCmp cmp] [Inhabited β]
 end Const
 
 section BEq
+
 variable {m₁ m₂ : DTreeMap α β cmp} [∀ k, BEq (β k)] [LawfulEqCmp cmp] [TransCmp cmp]
 
 theorem Equiv.beq [∀ k, ReflBEq (β k)] (h : m₁ ~m m₂) : m₁ == m₂ :=
   Impl.Equiv.beq m₁.2 m₂.2 h.1
 
 theorem equiv_of_beq [∀ k, LawfulBEq (β k)] (h : m₁ == m₂) : m₁ ~m m₂ :=
-  ⟨@Impl.equiv_of_beq _ _ ⟨cmp⟩ m₁.1 m₂.1 _ _ _ _ m₁.2 m₂.2 h⟩
+  ⟨Impl.equiv_of_beq m₁.2 m₂.2 h⟩
 
-theorem Equiv.beq_congr {m₃ m₄ : DTreeMap α β cmp} : m₁ ~m m₃ → m₂ ~m m₄ → (m₁ == m₂) = (m₃ == m₄) := fun h1 h2 =>
-  @Impl.Equiv.beq_congr _ _ ⟨cmp⟩ m₁.1 m₂.1 _ _ _ m₃.1 m₄.1 m₁.2 m₂.2 m₃.2 m₄.2 h1.1 h2.1
+theorem Equiv.beq_congr {m₃ m₄ : DTreeMap α β cmp} (w₁ : m₁ ~m m₃) (w₂ : m₂ ~m m₄) : (m₁ == m₂) = (m₃ == m₄) :=
+  Impl.Equiv.beq_congr m₁.2 m₂.2 m₃.2 m₄.2 w₁.1 w₂.1
 
 end BEq
 
 section
+
 variable {β : Type v} {m₁ m₂ : DTreeMap α (fun _ => β) cmp} [BEq β]
 
-theorem Const.Equiv.beq [TransCmp cmp] [ReflBEq β] (h : m₁ ~m m₂) : DTreeMap.Const.beq m₁ m₂ := by
-  apply Impl.Const.Equiv.beq m₁.2 m₂.2 h.1
+theorem Const.Equiv.beq [TransCmp cmp] [ReflBEq β] (h : m₁ ~m m₂) : DTreeMap.Const.beq m₁ m₂ :=
+  Impl.Const.Equiv.beq m₁.2 m₂.2 h.1
 
 theorem Const.equiv_of_beq [TransCmp cmp] [LawfulEqCmp cmp] [LawfulBEq β] (h : Const.beq m₁ m₂) : m₁ ~m m₂ :=
-  ⟨@Impl.Const.equiv_of_beq α ⟨cmp⟩ β m₁.1 m₂.1 _ _ _ _ m₁.2 m₂.2 h⟩
+  ⟨Impl.Const.equiv_of_beq m₁.2 m₂.2 h⟩
 
-theorem Const.Equiv.beq_congr [TransCmp cmp] [LawfulEqCmp cmp] {m₃ m₄ : DTreeMap α (fun _ => β) cmp} : m₁ ~m m₃ → m₂ ~m m₄ → Const.beq m₁ m₂ = Const.beq m₃ m₄ := fun h1 h2 =>
-  @Impl.Const.Equiv.beq_congr α ⟨cmp⟩ β m₁.1 m₂.1 _ _ m₃.1 m₄.1 _ m₁.2 m₂.2 m₃.2 m₄.2 h1.1 h2.1
+theorem Const.Equiv.beq_congr [TransCmp cmp] {m₃ m₄ : DTreeMap α (fun _ => β) cmp} (w₁ : m₁ ~m m₃) (w₂ : m₂ ~m m₄) : Const.beq m₁ m₂ = Const.beq m₃ m₄ :=
+  Impl.Const.Equiv.beq_congr m₁.2 m₂.2 m₃.2 m₄.2 w₁.1 w₂.1
 
 end
 
