src/Std/Data/DTreeMap/Raw/Lemmas.lean
@@ -3050,8 +3050,8 @@ variable {m₁ m₂ : Raw α β cmp} [∀ k, BEq (β k)] [LawfulEqCmp cmp] [Tran
 theorem Equiv.beq [∀ k, ReflBEq (β k)] (h₁ : m₁.WF) (h₂ : m₂.WF) : m₁ ~m m₂ → beq m₁ m₂ :=
   fun h => Impl.Equiv.beq h₁ h₂ h.1
 
-theorem equiv_of_beq [∀ k, LawfulBEq (β k)] (h₁ : m₁.WF) (h₂ : m₂.WF) : beq m₁ m₂ = true → m₁ ~m m₂ :=
-  fun hyp => ⟨@Impl.equiv_of_beq _ _ ⟨cmp⟩ m₁.1 m₂.1 _ _ _ _ h₁.1 h₂.1 hyp⟩
+theorem equiv_of_beq [∀ k, LawfulBEq (β k)] (h₁ : m₁.WF) (h₂ : m₂.WF) : beq m₁ m₂ = true → m₁ ~m m₂ := fun hyp =>
+  let : Ord α := ⟨cmp⟩; ⟨Impl.equiv_of_beq h₁.1 h₂.1 hyp⟩
 
 theorem Equiv.beq_congr {m₃ m₄ : Raw α β cmp} (h₁ : m₁.WF) (h₂ : m₂.WF) (h₃ : m₃.WF) (h₄ : m₄.WF) :
     m₁ ~m m₃ → m₂ ~m m₄ → Raw.beq m₁ m₂ = Raw.beq m₃ m₄ :=
@@ -3066,9 +3066,9 @@ theorem Const.Equiv.beq [TransCmp cmp] [BEq β] [ReflBEq β] (h₁ : m₁.WF) (h
   fun h => Impl.Const.Equiv.beq h₁ h₂ h.1
 
 theorem Const.equiv_of_beq [TransCmp cmp] [LawfulEqCmp cmp] [BEq β] [LawfulBEq β] (h₁ : m₁.WF) (h₂ : m₂.WF) : beq m₁ m₂ = true → m₁ ~m m₂ :=
-  fun hyp => ⟨@Impl.Const.equiv_of_beq α ⟨cmp⟩ β m₁.1 m₂.1 _ _ _ _ h₁.1 h₂.1 hyp⟩
+  fun hyp => let : Ord α := ⟨cmp⟩; ⟨Impl.Const.equiv_of_beq h₁.1 h₂.1 hyp⟩
 
-theorem Const.Equiv.beq_congr [TransCmp cmp] [LawfulEqCmp cmp] [BEq β] {m₃ m₄ : Raw α (fun _ => β) cmp} (h₁ : m₁.WF) (h₂ : m₂.WF) (h₃ : m₃.WF) (h₄ : m₄.WF) :
+theorem Const.Equiv.beq_congr [TransCmp cmp] [BEq β] {m₃ m₄ : Raw α (fun _ => β) cmp} (h₁ : m₁.WF) (h₂ : m₂.WF) (h₃ : m₃.WF) (h₄ : m₄.WF) :
     m₁ ~m m₃ → m₂ ~m m₄ → Raw.Const.beq m₁ m₂ = Raw.Const.beq m₃ m₄ :=
   fun w1 w2 => Impl.Const.Equiv.beq_congr h₁ h₂ h₃ h₄ w1.1 w2.1
 
