src/Std/Data/TreeMap/Raw/Lemmas.lean
@@ -2015,15 +2015,14 @@ end Inter
 section
 variable {β : Type v} {m₁ m₂ : Raw α β cmp}
 
-theorem Const.Equiv.beq [TransCmp cmp] [BEq β] [ReflBEq β] (h₁ : m₁.WF) (h₂ : m₂.WF) : m₁ ~m m₂ → m₁ == m₂ :=
-  fun h => DTreeMap.Raw.Const.Equiv.beq h₁ h₂ h.1
+theorem Const.Equiv.beq [TransCmp cmp] [BEq β] [ReflBEq β] (h₁ : m₁.WF) (h₂ : m₂.WF) (h : m₁ ~m m₂) : m₁ == m₂ :=
+  DTreeMap.Raw.Const.Equiv.beq h₁ h₂ h.1
 
-theorem Const.equiv_of_beq [TransCmp cmp] [LawfulEqCmp cmp] [BEq β] [LawfulBEq β] (h₁ : m₁.WF) (h₂ : m₂.WF) : m₁ == m₂ → m₁ ~m m₂ :=
-  fun hyp => ⟨@DTreeMap.Raw.Const.equiv_of_beq α _ β m₁.1 m₂.1 _ _ _ _ h₁.1 h₂.1 hyp⟩
+theorem Const.equiv_of_beq [TransCmp cmp] [LawfulEqCmp cmp] [BEq β] [LawfulBEq β] (h₁ : m₁.WF) (h₂ : m₂.WF) (k : m₁ == m₂) : m₁ ~m m₂ :=
+  ⟨DTreeMap.Raw.Const.equiv_of_beq h₁.1 h₂.1 k⟩
 
-theorem Const.Equiv.beq_congr [TransCmp cmp] [LawfulEqCmp cmp] [BEq β] {m₃ m₄ : Raw α β cmp} (h₁ : m₁.WF) (h₂ : m₂.WF) (h₃ : m₃.WF) (h₄ : m₄.WF) :
-    m₁ ~m m₃ → m₂ ~m m₄ → (m₁ == m₂) = (m₃ == m₄) :=
-  fun w1 w2 => DTreeMap.Raw.Const.Equiv.beq_congr h₁ h₂ h₃ h₄ w1.1 w2.1
+theorem Const.Equiv.beq_congr [TransCmp cmp] [BEq β] {m₃ m₄ : Raw α β cmp} (h₁ : m₁.WF) (h₂ : m₂.WF) (h₃ : m₃.WF) (h₄ : m₄.WF) (w₁ : m₁ ~m m₃) (w₂ : m₂ ~m m₄) : (m₁ == m₂) = (m₃ == m₄) :=
+  DTreeMap.Raw.Const.Equiv.beq_congr h₁ h₂ h₃ h₄ w₁.1 w₂.1
 
 end
 
