src/Std/Data/TreeSet/Raw/Lemmas.lean
@@ -816,15 +816,14 @@ end Inter
 section
 variable {m₁ m₂ : Raw α cmp}
 
-theorem Equiv.beq [TransCmp cmp] (h₁ : m₁.WF) (h₂ : m₂.WF) : m₁ ~m m₂ → beq m₁ m₂ := fun hyp =>
-  @TreeMap.Raw.Const.Equiv.beq _ cmp _ m₁.1 m₂.1 _ _ _ h₁ h₂ hyp.1
+theorem Equiv.beq [TransCmp cmp] (h₁ : m₁.WF) (h₂ : m₂.WF) (h : m₁ ~m m₂) : beq m₁ m₂ :=
+  TreeMap.Raw.Const.Equiv.beq h₁ h₂ h.1
 
-theorem equiv_of_beq [TransCmp cmp] [LawfulEqCmp cmp] (h₁ : m₁.WF) (h₂ : m₂.WF) : m₁ == m₂ → m₁ ~m m₂ := fun hyp =>
-  ⟨@TreeMap.Raw.Const.equiv_of_beq α cmp _ m₁.1 m₂.1 _ _ _ _ h₁.1 h₂.1 hyp⟩
+theorem equiv_of_beq [TransCmp cmp] [LawfulEqCmp cmp] (h₁ : m₁.WF) (h₂ : m₂.WF) (h : m₁ == m₂): m₁ ~m m₂ :=
+  ⟨TreeMap.Raw.Const.equiv_of_beq h₁.1 h₂.1 h⟩
 
-theorem Equiv.beq_congr [TransCmp cmp] [LawfulEqCmp cmp] {m₃ m₄ : Raw α cmp} (h₁ : m₁.WF) (h₂ : m₂.WF) (h₃ : m₃.WF) (h₄ : m₄.WF) :
-    m₁ ~m m₃ → m₂ ~m m₄ → (m₁ == m₂) = (m₃ == m₄) := fun hyp1 hyp2 =>
-  @TreeMap.Raw.Const.Equiv.beq_congr α cmp _ m₁.1 m₂.1 _ _ _ m₃.1 m₄.1 h₁.1 h₂.1 h₃.1 h₄.1 hyp1.1 hyp2.1
+theorem Equiv.beq_congr [TransCmp cmp] {m₃ m₄ : Raw α cmp} (h₁ : m₁.WF) (h₂ : m₂.WF) (h₃ : m₃.WF) (h₄ : m₄.WF) (w₁ : m₁ ~m m₃) (w₂ : m₂ ~m m₄) : (m₁ == m₂) = (m₃ == m₄) :=
+  TreeMap.Raw.Const.Equiv.beq_congr h₁.1 h₂.1 h₃.1 h₄.1 w₁.1 w₂.1
 
 end
 
